Also index typing judgement

theories/Dot/typing.v
@@ -1,7 +1,7 @@
 From D Require Import tactics.
 From D.Dot Require Import dotsyn.
 
-Reserved Notation "Γ ⊢ₜ e : T" (at level 74, e, T at next level).
+Reserved Notation "Γ ⊢ₜ e : T , i" (at level 74, e, T at next level).
 Reserved Notation "Γ ⊢ₚ p : T , i" (at level 74, p, T, i at next level).
 Reserved Notation "Γ ⊢ { l = d } : T" (at level 64, l, d, T at next level).
 Reserved Notation "Γ ⊢ds ds : T" (at level 74, ds, T at next level).
@@ -11,58 +11,57 @@ Implicit Types (L T U: ty) (v: vl) (e: tm) (d: dm) (ds: dms) (Γ : list ty).
 
 (**
 Judgments for typing, subtyping, path and definition typing.
-TODO: index the typing judgment as well.
-Here we follow Amin's judgment for definition typing: it is Γ ⊢ { l = d } : T,
+Here we follow Nada Amin's judgment for definition typing: it is Γ ⊢ { l = d } : T,
 meaning: this definition, with label l, has type T.
 This works, but requires reformulating again a bit semantic definition typing for proofs.
 *)
-Inductive typed Γ: tm → ty → Prop :=
+Inductive typed Γ: tm → ty → nat → Prop :=
 (** First, elimination forms *)
 (** Dependent application; only allowed if the argument is a value . *)
-| Appv_typed e1 v2 T1 T2 :
-    Γ ⊢ₜ e1: TAll T1 T2 →                        Γ ⊢ₜ tv v2 : T1 →
+| Appv_typed e1 v2 T1 T2 i:
+    Γ ⊢ₜ e1: TAll T1 T2, i →                        Γ ⊢ₜ tv v2 : T1, i →
     (*────────────────────────────────────────────────────────────*)
-    Γ ⊢ₜ tapp e1 (tv v2) : T2.|[v2/]
+    Γ ⊢ₜ tapp e1 (tv v2) : T2.|[v2/], i
 (** Non-dependent application; allowed for any argument. *)
-| App_typed e1 e2 T1 T2 :
-    Γ ⊢ₜ e1: TAll T1 T2.|[ren (+1)] →      Γ ⊢ₜ e2 : T1 →
+| App_typed e1 e2 T1 T2 i:
+    Γ ⊢ₜ e1: TAll T1 T2.|[ren (+1)], i →      Γ ⊢ₜ e2 : T1, i →
     (*────────────────────────────────────────────────────────────*)
-    Γ ⊢ₜ tapp e1 e2 : T2
-| Proj_typed e T l:
-    Γ ⊢ₜ e : TVMem l T →
+    Γ ⊢ₜ tapp e1 e2 : T2, i
+| Proj_typed e T l i:
+    Γ ⊢ₜ e : TVMem l T, i →
     (*─────────────────────────*)
-    Γ ⊢ₜ tproj e l : T
-| TMuE_typed v T:
-    Γ ⊢ₜ tv v: TMu T →
+    Γ ⊢ₜ tproj e l : T, i
+| TMuE_typed v T i:
+    Γ ⊢ₜ tv v: TMu T, i →
     (*──────────────────────*)
-    Γ ⊢ₜ tv v: T.|[v/]
+    Γ ⊢ₜ tv v: T.|[v/], i
 (** Introduction forms *)
 | Lam_typed e T1 T2 :
     (* T1 :: Γ ⊢ₜ e : T2 → (* Would work, but allows the argument to occur in its own type. *) *)
-    T1.|[ren (+1)] :: Γ ⊢ₜ e : T2 →
+    T1.|[ren (+1)] :: Γ ⊢ₜ e : T2, 0 →
     (*─────────────────────────*)
-    Γ ⊢ₜ tv (vabs e) : TAll T1 T2
+    Γ ⊢ₜ tv (vabs e) : TAll T1 T2, 0
 | VObj_typed ds T:
-    TLater T :: Γ ⊢ds ds: T →
+    (TLater T :: Γ) ⊢ds ds: T →
     (*──────────────────────*)
-    Γ ⊢ₜ tv (vobj ds): TMu T
-| TMuI_typed v T:
-    Γ ⊢ₜ tv v: T.|[v/] →
+    Γ ⊢ₜ tv (vobj ds): TMu T, 0
+| TMuI_typed v T i:
+    Γ ⊢ₜ tv v: T.|[v/], i →
     (*──────────────────────*)
-    Γ ⊢ₜ tv v: TMu T
+    Γ ⊢ₜ tv v: TMu T, i
 | Nat_typed n:
-    Γ ⊢ₜ tv (vnat n) : TNat
+    Γ ⊢ₜ tv (vnat n): TNat, 0
 
 (** "General" rules *)
 | Var_typed x T :
     (* After looking up in Γ, we must weaken T for the variables on top of x. *)
     Γ !! x = Some T →
     (*──────────────────────*)
-    Γ ⊢ₜ tv (var_vl x) : T.|[ren (+x)]
-| Subs_typed e T1 T2 :
-    Γ ⊢ₜ T1, 0 <: T2, 0 → Γ ⊢ₜ e : T1 →
+    Γ ⊢ₜ tv (var_vl x) : T.|[ren (+x)], 0
+| Subs_typed e T1 T2 i j :
+    Γ ⊢ₜ T1, i <: T2, j → Γ ⊢ₜ e : T1, i →
     (*───────────────────────────────*)
-    Γ ⊢ₜ e : T2
+    Γ ⊢ₜ e : T2, j
 (* XXX Must be generalized to something like the following, but that needs either
    skip instructions, or an indexed typing judgment. *)
 (* | Subs_typed e i1 i2 T1 T2 : *)
@@ -71,10 +70,10 @@ Inductive typed Γ: tm → ty → Prop :=
 (*     Γ ⊢ₜ e : T2 *)
 (* A bit surprising this is needed, but appears in the DOT papers, and this is
    only admissible if t has a type U that is a proper subtype of TAnd T1 T2. *)
-| TAndI_typed T1 T2 t:
-    Γ ⊢ₜ t : T1 →
-    Γ ⊢ₜ t : T2 →
-    Γ ⊢ₜ t : TAnd T1 T2
+| TAndI_typed T1 T2 t i:
+    Γ ⊢ₜ t : T1, i →
+    Γ ⊢ₜ t : T2, i→
+    Γ ⊢ₜ t : TAnd T1 T2, i
 with dms_typed Γ: dms → ty → Prop :=
 | dnil_typed : Γ ⊢ds [] : TTop
 | dcons_typed l d ds T1 T2 :
@@ -91,12 +90,12 @@ with dm_typed Γ : label → dm → ty → Prop :=
     Γ ⊢ₜ T, 1 <: U, 1 →
     Γ ⊢ { l = dtysyn T } : TTMem l L U
 | dvl_typed l v T:
-    Γ ⊢ₜ tv v : TLater T →
+    Γ ⊢ₜ tv v : TLater T, 0 →
     Γ ⊢ { l = dvl v } : TVMem l T
 with path_typed Γ: path → ty → nat → Prop :=
-| pv_typed v T :
-    Γ ⊢ₜ tv v : T →
-    Γ ⊢ₚ pv v : T, 0
+| pv_typed v T i:
+    Γ ⊢ₜ tv v : T, i →
+    Γ ⊢ₚ pv v : T, i
 (* Mnemonic: Path from SELecting a Field *)
 | pself_typed p T i l:
     Γ ⊢ₚ p : T, i →
@@ -192,7 +191,7 @@ with subtype Γ : ty → nat → ty → nat → Prop :=
     Γ ⊢ₜ U1, S i <: U2, S i →
     Γ ⊢ₜ TTMem l L1 U1, i <: TTMem l L2 U2, i
 
-where "Γ ⊢ₜ e : T" := (typed Γ e T)
+where "Γ ⊢ₜ e : T , i" := (typed Γ e T i)
 and "Γ ⊢ₚ p : T , i" := (path_typed Γ p T i)
 and "Γ ⊢ds ds : T" := (dms_typed Γ ds T)
 and "Γ ⊢ { l = d } : T" := (dm_typed Γ l d T)
